\section{Other}
\subsection{Bayes}
\begin{math}
  P(A|B) = \frac{P(A\cap B)}{P(B)}\ and\ P(B|A)
         = \frac{P(A\cap B)}{P(A)}
         \Rightarrow P(A\cap B) = P(A|B)P(B) = P(B|A)P(A)
         \Rightarrow P(A|B) = \frac{P(B|A)P(A)}{P(B)}
\end{math} \\[2pt]

\subsection{Marginal distribution}
\begin{math}
  f_X(x) = P(X = x)
         = P(\bigcup_y \{X = x, Y = y\})
         = \sum_y \left[ P(X = x, Y = y) \right]
         = \sum_y \left[ f_{XY}(x, y) \right]
\end{math} \\[2pt]

\subsection{Bernoulli}
\(Y = 1\) if successes otherwise 0 with probability \(p\) and \((1 - p)\) \\[2pt]
\begin{math}
  \expect{Y} = p,
  \expect{Y^2} = p
\end{math} \\[2pt]
\begin{math}
    Var(Y) = \expect{Y^2} - \expect{Y}^2 = p - p^2 = p(1 - p)
\end{math} \\[2pt]
\begin{math}
    X = \sum_{i = 1}^n Y_i, X \sim Bin(n, p)
    \Rightarrow
    \expect{X} = \expect{\sum_{i = 1}^n Y_i}
               = \sum_{i = 1}^n \expect{Y_i}
               = \sum_{i = 1}^n p
               = np
\end{math} \\[2pt]
\begin{math}
    Var(X) = Var(\sum_{i = 1}^n Var(Y_i) )
           = \sum_{i = 1}^n p(1 - p)
           = np(1 - p)
\end{math} \\[2pt]

\subsection{Estimators}
\subsubsection{Unbiased}
\begin{math}
  \hat{\theta} \text{ is unbiased if } \expect{\hat{\theta}} = \theta,
  \bar{X} = \frac{1}{n} \sum_{i = 1}^n X_i,
  \expect{\bar{X}} = \frac{1}{n} \sum_{i = 1}^n \expect{X_i} = \mu
\end{math} \\[2pt]
\subsubsection{Variance}
Proof for the computational formula: \\
\begin{math}
  S^2 = \frac{1}{n-1} \left[ \sum\limits_{i=1}^n \left[ X_i - \bar{X} \right]^2 \right]
      = \frac{1}{n-1} \left[ \sum\limits_{i=1}^n X_i^2 - 2X_i\bar{X} + \bar{X}^2 \right]
      = \frac{1}{n-1} \left[ \sum\limits_{i=1}^n X_i^2 - 2\sum\limits_{i=1}^n X_i\bar{X} + \sum\limits_{i=1}^n \bar{X}^2 \right]
      = \frac{1}{n-1} \left[ \sum\limits_{i=1}^n X_i^2 - 2\bar{X} \sum\limits_{i=1}^n X_i + n\bar{X}^2 \right]
      = \frac{1}{n-1} \left[ \sum\limits_{i=1}^n X_i^2 - \frac{2}{n} \left[ \sum\limits_{i=1}^n X_i \right]^2 + \frac{n}{n^2} \left[ \sum\limits_{i=1}^n X_i \right]^2 \right]
      = \frac{1}{n-1} \left[ \sum\limits_{i=1}^n X_i^2 - \frac{2}{n} \left[ \sum\limits_{i=1}^n X_i \right]^2 + \frac{1}{n} \left[ \sum\limits_{i=1}^n X_i \right]^2 \right]
      = \frac{1}{n-1} \left[ \sum\limits_{i=1}^n X_i^2 - \frac{1}{n} \left[ \sum\limits_{i=i}^n X_i \right]^2 \right]
\end{math} \\[2pt]
Note that \(S^2\) is also unbiased while \(S\) is biased, because math.
