\section{Probability}
\begin{math}
  P(\emptyset) = 0, P(\Omega) = 1,
  P(A^c) = 1 - P(A),
  A^c \cup A = \Omega
\end{math} \\[2pt]
\begin{math}
  P(A^c) + P(A) = P(A^c \cup A) = P(\Omega) = 1
\end{math} \\[2pt]
\begin{math}
  P(A \cup B) = P(A) + P(B) - P(A \cap B)
\end{math} \\[2pt]
\begin{math}
  P(A) = P(A \cap B^c) + P(A \cap B) + P(A^c \cap B) + P(A \cap B) = P(A \cup B) + P(A \cap B)
\end{math} \\[2pt]
\begin{math}
  P(A|B) = \frac{P(A \cap B)}{P(B)}
\end{math} \\[0pt]
A, B independent if
\begin{math}
  P(A \cap B) = P(A) \cdot P(B)
\end{math} \\[2pt]
Bayes:
\begin{math}
  P(A|B) = \frac{P(B|A) \cdot P(A)}{P(B)}
\end{math} \\[2pt]
Total Probability Law:
\begin{math}
  P(B) = \sum_i \left[P(B|A_i) \cdot P(A_i)\right]
\end{math} \\[2pt]
